theories/RTac/CoreK.v
@@ -1,0 +1,128 @@
+Require Import Coq.Classes.Morphisms.
+Require Import Coq.Relations.Relations.
+Require Import ExtLib.Core.RelDec.
+Require Import ExtLib.Structures.Monad.
+Require Import ExtLib.Structures.Traversable.
+Require Import ExtLib.Data.Option.
+Require Import ExtLib.Data.Prop.
+Require Import ExtLib.Data.Pair.
+Require Import ExtLib.Data.List.
+Require Import ExtLib.Data.HList.
+Require Import ExtLib.Data.Monads.OptionMonad.
+Require Import ExtLib.Tactics.
+Require Import MirrorCore.ExprI.
+Require Import MirrorCore.SubstI.
+Require Import MirrorCore.ExprDAs.
+Require Import MirrorCore.RTac.Core.
+
+Require Import MirrorCore.Util.Quant.
+Require Import MirrorCore.Util.Forwardy.
+
+Set Implicit Arguments.
+Set Strict Implicit.
+
+Section parameterized.
+  Variable typ : Type.
+  Variable expr : Type.
+  Variable subst : Type.
+
+  Context {RType_typ : RType typ}.
+  Context {Expr_expr : Expr RType_typ expr}.
+  Context {Typ0_Prop : Typ0 _ Prop}.
+  Context {Subst_subst : Subst subst expr}.
+  Context {SubstOk_subst : @SubstOk _ _ _ _ Expr_expr Subst_subst}.
+  Context {SubstUpdate_subst : SubstUpdate subst expr}.
+  Context {SubstUpdateOk_subst : @SubstUpdateOk _ _ _ _ Expr_expr Subst_subst _ _}.
+
+  Definition rtacK_spec tus tvs ctx (s : ctx_subst subst ctx) (g : Goal _ _)
+             (r : Result _ ctx) : Prop :=
+    match r with
+      | Fail => True
+      | Solved s' =>
+        WellFormed_ctx_subst s ->
+        WellFormed_ctx_subst s' /\
+        match pctxD tus tvs s
+            , goalD _ _ g
+            , pctxD tus tvs s'
+        with
+          | None , _ , _
+          | Some _ , None , _ => True
+          | Some _ , Some _ , None => False
+          | Some cD , Some gD , Some cD' =>
+            SubstMorphism tus tvs s s' /\
+            forall us vs, cD' gD us vs
+        end
+      | More_ s' g' =>
+        WellFormed_ctx_subst s ->
+        WellFormed_ctx_subst s' /\
+        match pctxD tus tvs s
+            , goalD _ _ g
+            , pctxD tus tvs s'
+            , goalD _ _ g'
+        with
+          | None , _ , _ , _
+          | Some _ , None , _ , _ => True
+          | Some _ , Some _ , None , _
+          | Some _ , Some _ , Some _ , None => False
+          | Some cD , Some gD , Some cD' , Some gD' =>
+            SubstMorphism tus tvs s s' /\
+            forall us vs,
+              cD' (fun us vs => gD' us vs -> gD us vs) us vs
+        end
+    end.
+
+  Theorem Proper_rtacK_spec tus tvs ctx s
+  : Proper (EqGoal (tus ++ getUVars ctx) (tvs ++ getVars ctx) ==>
+            @EqResult _ _ _ _ _ _ (tus ++ getUVars ctx) (tvs ++ getVars ctx) ctx
+            ==> iff)
+           (@rtacK_spec tus tvs ctx s).
+  Proof.
+    red. red. red.
+    unfold rtacK_spec.
+    inversion 2.
+    { destruct x0; destruct y0; simpl in *; try congruence.
+      reflexivity. }
+    { destruct x0; destruct y0; simpl in *;
+      try solve [ reflexivity | congruence ]; inv_all; subst; inv_all;
+      try (eapply impl_iff; try reflexivity; intros;
+           eapply and_iff; try reflexivity; intros;
+           try inversion H; try reflexivity;
+           try inversion H5; try reflexivity;
+           repeat match goal with
+                    | |- context [ match ?X with _ => _ end ] =>
+                      consider X; intros; try reflexivity; [ ]
+                  end;
+           eapply and_iff; try reflexivity; intros;
+           do 2 (eapply forall_iff; intro);
+           eapply Fmap_pctxD_iff; eauto; try reflexivity;
+           do 5 red; intros).
+      { apply impl_iff; [ eapply H10; eauto | intro ].
+        apply H7; eauto. }
+      { do 5 red in H10.
+        rewrite H10; try reflexivity.
+        rewrite True_impl_iff.
+        eapply H7; eauto. }
+      { do 5 red in H10.
+        rewrite <- H10; try reflexivity.
+        rewrite True_impl_iff.
+        eapply H7; eauto. } }
+  Qed.
+
+  (** Treat this as opaque! **)
+  Definition rtacK : Type :=
+    tenv typ -> tenv typ -> nat -> nat ->
+    forall c : Ctx typ expr, ctx_subst subst c -> Goal typ expr -> Result subst c.
+
+  Definition rtacK_sound (tus tvs : tenv typ) (tac : rtacK)
+  : Prop :=
+    forall ctx s g result,
+      (let tus := tus ++ getUVars ctx in
+       let tvs := tvs ++ getVars ctx in
+       tac tus tvs (length tus) (length tvs) ctx s g = result) ->
+      @rtacK_spec tus tvs ctx s g result.
+
+End parameterized.
+
+Export MirrorCore.ExprI.
+Export MirrorCore.SubstI.
+Export MirrorCore.ExprDAs.
