theories/RTac/RTac.v
@@ -1,4 +1,6 @@
 Require Export MirrorCore.RTac.Core.
+Require Export MirrorCore.RTac.CoreK.
+
 Require Export MirrorCore.RTac.Idtac.
 Require Export MirrorCore.RTac.Fail.
 Require Export MirrorCore.RTac.First.
@@ -15,5 +17,3 @@ Require Export MirrorCore.RTac.Simplify.
 Require Export MirrorCore.RTac.Instantiate.
 (*Require Export MirrorCore.RTac.RunSTac.*)
 Require Export MirrorCore.RTac.AtGoal.
-
-Require Export MirrorCore.RTac.CoreGlobal.
